lib/hst/Hacl.UInt128.fst
@@ -1,38 +1,130 @@
 module Hacl.UInt128
+(* This module generated automatically using [mk_int.sh] *)
 
-open FStar.Mul
 open FStar.UInt128
+module U = FStar.UInt128
+open FStar.Mul
 
-module U128 = FStar.UInt128
+(* NOTE: anything that you fix/update here should be reflected in [Hacl.IntN.fstp], which is mostly
+ * a copy-paste of this module. *)
 
-private type _t = U128.t
-type t = _t
+let n = U.n
 
-let n = n
+private type t' = | Mk: v:U.t -> t'
+type t = t'
 
-let v (a:t) : GTot int = v a
-let add = add
-let add_underspec = add_underspec
-let add_mod = add_mod
-let sub = sub
-let sub_underspec = sub_underspec
-let sub_mod = sub_mod
-let mul = mul
-let mul_underspec = mul_underspec
-let mul_mod = mul_mod
-assume val mul_wide: a:Hacl.UInt64.t -> b:Hacl.UInt64.t -> Tot (c:t{(v c = Hacl.UInt64.v a * Hacl.UInt64.v b)})
-let div = div
-let div_underspec = div_underspec
-let rem = rem
-let logand = logand
-let logor = logor
-let logxor = logxor
-let lognot = lognot
-let shift_right = shift_right
-let shift_left = shift_left
-assume val eq_mask: a:t -> b:t -> Tot (c:t{(v a = v b <==> v c = pow2 n - 1) /\ (v a <> v b <==> v c = 0)})
-assume val gte_mask: a:t -> b:t -> Tot (c:t{(v a >= v b <==> v c = pow2 n - 1) /\ (v a < v b <==> v c = 0)})
-assume val lt_mask: a:t -> b:t -> Tot (c:t{(v a < v b <==> v c = pow2 n - 1) /\ (v a >= v b <==> v c = 0)})
+let v (x:t) : GTot (FStar.UInt.uint_t n) = U.v x.v
+
+val add: a:t -> b:t -> Pure t
+  (requires (UInt.size (v a + v b) n))
+  (ensures (fun c -> v a + v b = v c))
+let add a b =
+  Mk (add (a.v) (b.v))
+
+val add_underspec: a:t -> b:t -> Pure t
+  (requires True)
+  (ensures (fun c ->
+    UInt.size (v a + v b) n ==> v a + v b = v c))
+let add_underspec a b =
+  Mk (add_underspec (a.v) (b.v))
+
+val add_mod: a:t -> b:t -> Pure t
+  (requires True)
+  (ensures (fun c -> (v a + v b) % pow2 n = v c))
+let add_mod a b =
+  Mk (add_mod (a.v) (b.v))
+
+(* Subtraction primitives *)
+val sub: a:t -> b:t -> Pure t
+  (requires (UInt.size (v a - v b) n))
+  (ensures (fun c -> v a - v b = v c))
+let sub a b =
+  Mk (sub (a.v) (b.v))
+
+val sub_underspec: a:t -> b:t -> Pure t
+  (requires True)
+  (ensures (fun c ->
+    UInt.size (v a - v b) n ==> v a - v b = v c))
+let sub_underspec a b =
+  Mk (sub_underspec (a.v) (b.v))
+
+val sub_mod: a:t -> b:t -> Pure t
+  (requires True)
+  (ensures (fun c -> (v a - v b) % pow2 n = v c))
+let sub_mod a b =
+  Mk (sub_mod (a.v) (b.v))
+
+(* Multiplication primitives *)
+val mul: a:t -> b:t -> Pure t
+  (requires (UInt.size (v a * v b) n))
+  (ensures (fun c -> v a * v b = v c))
+let mul a b =
+  Mk (mul (a.v) (b.v))
+
+val mul_underspec: a:t -> b:t -> Pure t
+  (requires True)
+  (ensures (fun c ->
+    UInt.size (v a * v b) n ==> v a * v b = v c))
+let mul_underspec a b =
+  Mk (mul_underspec (a.v) (b.v))
+
+val mul_mod: a:t -> b:t -> Pure t
+  (requires True)
+  (ensures (fun c -> (v a * v b) % pow2 n = v c))
+let mul_mod a b =
+  Mk (mul_mod (a.v) (b.v))
+
+(* Division primitives *)
+val div: a:t -> b:t{v b <> 0} -> Pure t
+  (requires (UInt.size (v a / v b) n))
+  (ensures (fun c -> v b <> 0 ==> v a / v b = v c))
+let div a b =
+  Mk (div (a.v) (b.v))
+
+val div_underspec: a:t -> b:t{v b <> 0} -> Pure t
+  (requires True)
+  (ensures (fun c ->
+    (v b <> 0 /\ UInt.size (v a / v b) n) ==> v a / v b = v c))
+let div_underspec a b =
+  Mk (div_underspec (a.v) (b.v))
+
+(* Modulo primitives *)
+val rem: a:t -> b:t{v b <> 0} -> Pure t
+  (requires True)
+  (ensures (fun c ->
+    v a - ((v a / v b) * v b) = v c))
+let rem a b = Mk (rem (a.v) (b.v))
+
+(* Bitwise operators *)
+val logand: t -> t -> Tot t
+let logand a b = Mk (logand (a.v) (b.v))
+val logxor: t -> t -> Tot t
+let logxor a b = Mk (logxor (a.v) (b.v))
+val logor: t -> t -> Tot t
+let logor a b = Mk (logor (a.v) (b.v))
+val lognot: t -> Tot t
+let lognot a = Mk (lognot (a.v))
+
+val uint_to_t: x:(UInt.uint_t n) -> Pure t
+  (requires True)
+  (ensures (fun y -> v y = x))
+let uint_to_t x = Mk (uint_to_t x)
+
+(* Shift operators *)
+val shift_right: a:t -> s:FStar.UInt32.t -> Pure t
+  (requires True)
+  (ensures (fun c -> FStar.UInt32.v s < n ==> v c = (v a / (pow2 (FStar.UInt32.v s)))))
+let shift_right a s = Mk (shift_right (a.v) s)
+
+val shift_left: a:t -> s:FStar.UInt32.t -> Pure t
+  (requires True)
+  (ensures (fun c -> FStar.UInt32.v s < n ==> v c = ((v a * pow2 (FStar.UInt32.v s)) % pow2 n)))
+let shift_left a s = Mk (shift_left (a.v) s)
+
+assume val eq_mask: a:t -> b:t -> Tot (c:t{(v a = v b ==> v c = pow2 n - 1) /\ (v a <> v b ==> v c = 0)})
+assume val gte_mask: a:t -> b:t -> Tot (c:t{(v a >= v b ==> v c = pow2 n - 1) /\ (v a < v b ==> v c = 0)})
+
+(* Infix notations *)
 let op_Plus_Hat = add
 let op_Plus_Question_Hat = add_underspec
 let op_Plus_Percent_Hat = add_mod
@@ -44,38 +136,15 @@ let op_Star_Question_Hat = mul_underspec
 let op_Star_Percent_Hat = mul_mod
 let op_Slash_Hat = div
 let op_Percent_Hat = rem
-let op_Hat_Hat = logxor  
+let op_Hat_Hat = logxor
 let op_Amp_Hat = logand
 let op_Bar_Hat = logor
 let op_Less_Less_Hat = shift_left
 let op_Greater_Greater_Hat = shift_right
-let op_Equal_Hat = eq
-let op_Greater_Hat = gt
-let op_Greater_Equal_Hat = gte
-let op_Less_Hat = gt
-let op_Less_Equal_Hat = gte
-type byte = t
 
-let op_Hat_Plus= add
-let op_Hat_Plus_Question= add_underspec
-let op_Hat_Plus_Percent= add_mod
-let op_Hat_Subtraction= sub
-let op_Hat_Subtraction_Question= sub_underspec
-let op_Hat_Subtraction_Percent= sub_mod
-let op_Hat_Star= mul
-let op_Hat_Star_Question= mul_underspec
-let op_Hat_Star_Percent= mul_mod
-let op_Hat_Slash= div
-let op_Hat_Percent= rem
-let op_Hat_Amp= logand
-let op_Hat_Bar= logor
-let op_Hat_Less_Less= shift_left
-let op_Hat_Greater_Greater= shift_right
-let op_Hat_Equal= eq
-let op_Hat_Greater= gt
-let op_Hat_Greater_Equal= gte
-let op_Hat_Less= gt
-let op_Hat_Less_Equal= gte
+(* To input / output constants *)
+assume val of_string: string -> Tot t
 
-let of_string = of_string
-let uint_to_t = uint_to_t
+assume val mul_wide: a:Hacl.UInt64.t -> b:Hacl.UInt64.t -> Pure t
+  (requires True)
+  (ensures (fun c -> v c = Hacl.UInt64.v a * Hacl.UInt64.v b))
