lib/hst/mk_int.sh
@@ -1,0 +1,26 @@
+#!/bin/bash
+
+# Taken from the FStar repository
+
+for i in 8 16 32 64 128; do
+  f=Hacl.UInt$i.fst
+  cat > $f <<EOF
+module Hacl.UInt$i
+(* This module generated automatically using [mk_int.sh] *)
+
+open FStar.UInt$i
+module U = FStar.UInt$i
+EOF
+  cat Hacl.UIntN.fstp >> $f
+  if [ $i -eq 8 ]; then
+    echo "type byte = t" >> $f
+  fi
+  if [ $i -eq 128 ]; then
+      cat >> $f <<EOF
+
+assume val mul_wide: a:Hacl.UInt64.t -> b:Hacl.UInt64.t -> Pure t
+  (requires True)
+  (ensures (fun c -> v c = Hacl.UInt64.v a * Hacl.UInt64.v b))
+EOF
+  fi
+done
